src/UntypedComp2.v
@@ -68,6 +68,12 @@ Lemma compile_cu_compile_genv : forall A Ameta B Bmeta,
 simpl. inversion 1. auto.
 Qed.
 
+Lemma compile_cu_metas : forall A Ameta B Bmeta,
+    compile_cu (A, Ameta) = (B, Bmeta) ->
+    Ameta = Bmeta.
+simpl. inversion 1. auto.
+Qed.
+
 Lemma compile_genv_length : forall a,
     length a = length (compile_genv a).
 induction a; simpl in *.
@@ -103,6 +109,7 @@ Section Preservation.
     Theorem fsim : Semantics.forward_simulation (A.semantics aprog) (B.semantics bprog).
     destruct aprog as [A Ameta], bprog as [B Bmeta].
     fwd eapply compile_cu_compile_genv; eauto.
+    fwd eapply compile_cu_metas; eauto.
 
     eapply Semantics.forward_simulation_step with
         (match_states := @eq S.state)
